# Lab 1

Link to raw file: 

[Lab 1](https://www.notion.so/Lab-1-0f6753fb79724f25a82b35549eb90d3a?pvs=21)

Original HW PDF:

[Lab 1.pdf](Lab%201%200f6753fb79724f25a82b35549eb90d3a/Lab_1.pdf)

> Jacob Ursenbach
CSCI 420
Prof: Dr. Jaime Raigoza 
20230606
> 

# LaTex References:

${\sqrt{-1} \over {3+\sqrt{-1}}}+3$ - fractions and sqrt - {\sqrt{-1} \over {3+\sqrt{-1}}}+3

$\begin{bmatrix} 1 & 2 \\ 3 & 4\end{bmatrix}$ - matrix - \begin{bmatrix} 1 & 2 \\ 3 & 4\end{bmatrix}

$\overline{M}$ or $M^*$ - conjugate of - \overline{M} or M^*

$\dagger$ - dagger - \dagger

$\lang c_1 \otimes c_2 \rang$ -  tensor (or **Kronecker) product**  - \lang c_1 \otimes c_2 \rang

---

## Formulas:

<aside>
‚ùï **Objective:**

1. Complete the following problems. Rather than hand-written, try to use a nice professional tool such as LaTeX or Microsoft Equation that professionally makes the brackets which completely encompass multi-dimensional matrices. However, scanned hand-written work is ok but ensure it is legible.
2. For all problems, ensure that your work is shown.
</aside>

---

# 1. (1.1) ‚úÖ

> ‚ùì Come up with two equations that have no solution with real numbers. However, the equation should have a solution with complex numbers. Make sure to solve the equation. For example, an equation is $ùë•^2+1=0$ and it is solved as $ùë•^2=‚àí1$,hence $ùë•=ùëñ$. ‚ùì
> 

## Equation 1:

$2x^2+1 =0 \\ 
\rightarrow x^2= - {1 \over 2} \\
x = \pm {1 \over \sqrt{2}}i$

## Equation 2:

$x^2 + 2 = 0 \\ 
\rightarrow x^2 = -2 \\
\rightarrow x = \pm \sqrt{2}i$

## Answer:

<aside>
‚úÖ Equation 1:

$$
2x^2+1 = 0
\;\;\;\;\;\;\bigg|\;\;\;\;\;\; 
x = \pm{1 \over \sqrt{2}}i
$$

Equation 2: 

$$
x^2+2=0 
\;\;\;\;\;\; \bigg | \;\;\;\;\;\;
x = \pm \sqrt{2}i
$$

</aside>

---

# 2. (1.2.3)  ‚úÖ

> ‚ùì Given $c_1 = 5 + 3i$ and $c_2 = 9 ‚Äì 2i$, calculate $c_1 \over c_2$. ‚ùì
> 

<aside>
‚ÑπÔ∏è FORMULA:

$$
{c_1 \over c_2} = 
{a_1+b_1i \over a_2 + b_2i} =  
{{a_1a_2+b_1b_2} \over {a_2^2+b_2^2}}+ {{a_2b_1 - a_1b_2}\over{a_2^2+b_2^2}}i
$$

> Note: the denominator is $(a+bi)_2^2$, but if you foil that out, it becomes equal to $a_2^2+b_2^2$, the i goes away since $(\sqrt{-1})^2 = -1$
> 
</aside>

$$
{5 + 3i \over 9-2i} = {5(9)+3(-2) \over 9^2+2^2}+{9(3i)-5(-2i) \over 9^2+2^2}
$$

<aside>
üí° alternative method:

$$
 {(45+10i+27i+6i^2) \over (81+18i-18i-4i^2)}
$$

</aside>

$$
{45-6+27i+10i \over 81-4} = {39+37i \over 85} = {1 \over 85}(39+37i)
$$

## Answer:

<aside>
‚úÖ $C_1 / C_2 =$

$$
{1 \over 85}(39+37i)
$$

</aside>

# 3. (1.2.3) ‚úÖ

> ‚ùì What is the modulus of 7 - 2i? ‚ùì
> 

<aside>
‚ÑπÔ∏è Formula:
x is the real part and y is the imaginary part of the complex number

$$
z=\sqrt{x^2 + y^2}
$$

</aside>

$$
z = \sqrt{7^2 + (-2i)^2}=\sqrt{49+4} = \sqrt{53}
$$

## Answer:

<aside>
‚úÖ The modulus of 7-2i =

$$
\sqrt{53}
$$

</aside>

# 4. (1.3.2) ‚ùì

> ‚ùì What is the polar representation of $5 + 3i?$
Draw it using a similar figure as Figure 1.5 from the textbook using degrees to measure the angle. ‚ùì
> 

<aside>
‚ÑπÔ∏è Formula:

the polar representation $(p,\theta)$ for a complex number a+bi $(a,b)$:

$$
p=\sqrt{a^2+b^2} \\
\theta = tan^{-1}(b/a)
$$

</aside>

## Finding r:

$$
p=\sqrt{5^2+(3i)^2} \\
p=\sqrt{25+ (-9) } \\
p=\sqrt{16 } \\
p=4
$$

## Finding $\theta$:

$$
\theta = tan^{-1}({3/5}) \approx 30.96\degree
$$

## Picture Representation for $(4,30\degree)$:

![Untitled](Lab%201%200f6753fb79724f25a82b35549eb90d3a/Untitled.png)

## Answer:

<aside>
‚úÖ polar: $(4,30\degree)$

![Untitled](Lab%201%200f6753fb79724f25a82b35549eb90d3a/Untitled.png)

</aside>

---

# 5. (2.2.1) ‚ùì

> ‚ùì Let $R_1 = 4$, $R_2 = 5$, and $V = \begin{bmatrix} 2 \\ -3 \\ 6 \end{bmatrix}$, 
verify the property (vi) from page 34 of our textbook. 

Show that $r_1 *(r_2*V)$  and $(r_1 * r_2) * V$ coincide.
> 

<aside>
‚ÑπÔ∏è Property (vi) on page 34:

*Scalar multiplication respects complex multiplication:*

$$
c_1 \cdot (c_2 \cdot C) = (C_1 \times c_2) \cdot V
$$

</aside>

$r_1 = 4\\r_2 = 5\\
V = \begin{bmatrix}
2\\-3\\6
\end{bmatrix}$

## <left side>  $r_1 *(r_2*V)$   :

$$
4 * \bigg(5 * \begin{bmatrix}
2\\-3\\6
\end{bmatrix}\bigg) = 4 * \bigg( 
 \begin{bmatrix}
10\\-15\\30
\end{bmatrix}
\bigg) = \begin{bmatrix}
40\\-60\\120
\end{bmatrix}
$$

## <right side> $(r_1 * r_2) * V$ :

$$
\bigg( 4 * 5 \bigg) * \begin{bmatrix}
2\\-3\\6
\end{bmatrix} = \bigg( 20 \bigg) * \begin{bmatrix}
2\\-3\\6
\end{bmatrix} =  \begin{bmatrix}
40\\-60\\120
\end{bmatrix}
$$

## Verify sides are equal :

$$
4 * \bigg(5 * \begin{bmatrix}
2\\-3\\6
\end{bmatrix}\bigg) = \begin{bmatrix}
40\\-60\\120
\end{bmatrix} \\
$$

$$
\bigg( 4 * 5 \bigg) * \begin{bmatrix}
2\\-3\\6
\end{bmatrix}= \begin{bmatrix}
40\\-60\\120
\end{bmatrix} \\   
$$

$$
4 * \bigg(5 * \begin{bmatrix}
2\\-3\\6
\end{bmatrix}\bigg) = \begin{bmatrix}
40\\-60\\120
\end{bmatrix} = \bigg( 4 * 5 \bigg) * \begin{bmatrix}
2\\-3\\6
\end{bmatrix}
$$

## Answer:

<aside>
‚úÖ The two sides are equal, therefore property (vi) from page 34 has been verified (but not proven):

$$
4 * \bigg(5 * \begin{bmatrix}
2\\-3\\6
\end{bmatrix}\bigg) = \begin{bmatrix}
40\\-60\\120
\end{bmatrix} = \bigg( 4 * 5 \bigg) * \begin{bmatrix}
2\\-3\\6
\end{bmatrix}
$$

</aside>

---

# 6. (2.2.1) ‚ùì

> ‚ùì Let: 
$c_1 = 4i$
$c_2 = 2+3i$
$V = \begin{bmatrix}2-i & 4+2i \\ 3 & 1+i\end{bmatrix}$
 
Verify property (viii) from page 34 of our textbook in showing $\mathbb{C}^{2 x 2}$ is a complex vector space.
> 

<aside>
‚ÑπÔ∏è Property (viii) on page 34:

*Scalar multiplication distributes over complex addition:*

$$
V \cdot(c_1 + c_2)  = c_1 \cdot V + c_2 \cdot V
$$

</aside>

<aside>
‚ÑπÔ∏è formula for multiplying complex numbers:

$$
(a + ib) (c + id) = (ac - bd) + i(ad + bc)
$$

</aside>

## <left side> $V \cdot (c_1 + c_2)$ :

$$
\begin{bmatrix}2-i & 4+2i \\ 3 & 1+i\end{bmatrix} * \bigg(4i + (2+3i) \bigg)
$$

$$
\begin{bmatrix}2-i & 4+2i \\ 3 & 1+i\end{bmatrix} * (2+7i)
$$

$$
(2-i) * (2+7i) = 11 + 12i
$$

$$
(4+2i) * (2+7i) = -6 + 32i = 2(-3+16i)
$$

$$
 3* (2+7i) = 6+21i
$$

$$
(1+i) * (2+7i) = -5 + 9i
$$

### result:

There are two ways of writing this:

$$
\begin{bmatrix}
11+12i & 2(-3+16i)\\
3(2+7i) & -5+9i
\end{bmatrix}  or 
\begin{bmatrix}
11+12i & -6+32i)\\
6+21i) & -5+9i
\end{bmatrix} 
$$

## <right side> $c_1 \cdot V + c_2 \cdot V$ :

$$
4i\begin{bmatrix}2-i & 4+2i \\ 3 & 1+i\end{bmatrix} + (2+3i)\begin{bmatrix}2-i & 4+2i \\ 3 & 1+i\end{bmatrix}
$$

$$
4i * (2-i) = 4 + 8i= 4(1+2i)
$$

$$
4i * (4+2i)= -8 + 16i =8(-1 + 2i)
$$

$$
4i*3 =12 i
$$

$$
4i * (1+i)= 4i-1 = 4(-1+i)
$$

There are two ways of writing the resulting matrix: 

$$
\begin{bmatrix}
4+8i & -8+16i \\
12i & -4+4i
\end{bmatrix} or\begin{bmatrix}
4(1+2i) & 8(-1+2i) \\
12i & 4(-1+i)
\end{bmatrix}
$$

$$
(2+3i)*(2-i) = 7 + 4i
$$

$$
(2+3i)* (4+2i) = 2 + 16i = 2(1+8i)
$$

$$
(2+3i)* (3) = 6 + 9i = 3(2+3i)
$$

$$
(2+3i)* (1+i) = -1 + 5i
$$

There are two ways of writing the resulting matrix:

$$
\begin{bmatrix} 
7 + 4i & 2+16i)\\
6+9i & -1+5i
\end{bmatrix}
=
\begin{bmatrix} 
7 + 4i & 2(1+8i)\\
3(2+3i) & -1+5i
\end{bmatrix}
$$

### add the two matrices :

$$
\begin{bmatrix}
4+8i & -8+16i \\
12i & -4+4i
\end{bmatrix} + \begin{bmatrix} 
7 + 4i & 2+16i)\\
6+9i & -1+5i
\end{bmatrix} = 

\begin{bmatrix} 11 + 12i & -6 + 32i \\
6 + 14i & -5 + 9i
\end{bmatrix}
$$

there are two ways of writing this:

$$
\begin{bmatrix}
11+12i & 2(-3+16i)\\
3(2+7i) & -5+9i
\end{bmatrix}  or 
\begin{bmatrix}
11+12i & -6+32i)\\
6+21i) & -5+9i
\end{bmatrix} 
$$

## compare left and right side:

$$
\begin{bmatrix}
11+12i & -6+32i)\\
6+21i) & -5+9i
\end{bmatrix}  = \begin{bmatrix}
11+12i & -6+32i)\\
6+21i) & -5+9i
\end{bmatrix} 
$$

## Answer:

<aside>
‚úÖ The two sides are equal, verifying property (viii):

*Scalar multiplication distributes over complex addition:*

$$
\begin{bmatrix}
11+12i & -6+32i)\\
6+21i) & -5+9i
\end{bmatrix}  = \begin{bmatrix}
11+12i & -6+32i)\\
6+21i) & -5+9i
\end{bmatrix} 
$$

</aside>

---

# 7. (2.2.5) ‚ùì

> ‚ùì Find the conjugate transpose of the following matrix:
> 
> 
> $$
> \begin{bmatrix}
> i & 2+ i \\ 
> 5 & 5 \\
> 9+7i & -3 -3i
>  \end{bmatrix}
> $$
> 

<aside>
‚ÑπÔ∏è **Transpose:**

Interchange rows and columns 

EX:

$$
\begin{bmatrix} 
a & b & c \\ 
d & e & f \\ 
g & h & i \\
\end{bmatrix}^T =
 
\begin{bmatrix}
a & d & g \\ 
b & e & h \\ 
c & f & i \\
\end{bmatrix}
$$

**Conjugate:** 

Take the complex conjugate of each object in the matrix. 

To do this for each complex number switch the sign for the complex number

EX:

$$
\begin{bmatrix} 
a+bi & c-di\\  
e-fi & g+hi
\end{bmatrix}^* = \begin{bmatrix} 
a-bi & c+di\\  
e+fi & g-hi
\end{bmatrix}
$$

</aside>

## transpose:

$$
A^T = \begin{bmatrix}
i & 5 & 9+7i \\
2+ i & 5 & -3 -3i
\end{bmatrix}
$$

## conjugate:

$$
A^*= \overline A = \begin{bmatrix}
-i & 5 & 9-7i \\
2- i & 5 & -3 +3i
\end{bmatrix}
$$

## Answer:

<aside>
‚úÖ The conjugate transpose of the matrix:

$$
\overline{A}^T = A^\dagger=\begin{bmatrix}
-i & 5 & 9-7i \\
2- i & 5 & -3 +3i
\end{bmatrix}
$$

</aside>

---

# 8. (2.4.1) ‚ùì

> ‚ùì Given $V_1 = [5,1,2]^t$, $V_2 = [3,2,1]^t$, and $c=5$, show that the inner product respects the following multiplication equation:
> 
> 
> $$
> \lang c * V_1,V_2 \rang = c * \lang V_1,V_2 \rang
> $$
> 

<aside>
‚ÑπÔ∏è the inner product is a special version of the dot product.  

to calculate the inner product of two vectors add the products of the cooresponding components: 

EX: 

for two vectors v and w:

$$
‚ü®ùêØ, ùê∞‚ü© = ùêØ‚ÇÅùê∞‚ÇÅ + ùêØ‚ÇÇùê∞‚ÇÇ + ‚ãØ + ùêØ‚Çôùê∞‚Çô,
$$

</aside>

## <left side> $\lang c * V_1,V_2 \rang$

$$
c*V1 = 5 * [5,1,2]^t = [25,5,10]^t
$$

$$
 ‚ü®cV1, V2‚ü© = [25,5,10] ‚Ä¢ [3,2,1] = (253 + 52 + 10*1) = 95
$$

## <right side>  $c * \lang V_1,V_2 \rang$

$$
 ‚ü®V1, V2‚ü© = [5,1,2] ‚Ä¢ [3,2,1] = (53 + 12 + 2*1) = 19
$$

$$
 5 * 19 = 95
$$

## compare the two:

$$
\lang c * V_1,V_2 \rang = 95 \\
 c * \lang V_1,V_2 \rang = 95 \\ 
95 = 95
$$

## Answer:

<aside>
‚úÖ Because we have show that the two sides are equal to each other, we have shown that the inner product respects homogeneity of scalar multiplication.

$$
\lang c * V_1,V_2 \rang = 95 =
 c * \lang V_1,V_2 \rang
$$

</aside>

---

# 9. (2.4.7) ‚ùì

> ‚ùì Calculate the distance between these 2 vectors,
> 
> 
> $$
> V_1 = \begin{bmatrix}2 \\ 3 \\\ 1 \end{bmatrix} \text{ and } V_2 = \begin{bmatrix}-1 \\ 3 \\\ -2 \end{bmatrix}
> $$
> 

<aside>
‚ÑπÔ∏è To calculate the distance between two vectors you calculate  the magnitude of the difference of the vectors, annotated like this:

$$
||V_2 - V_1 || 
$$

This is achieved by taking the square root of the sum of the squares of the components of the difference:

$$
||A-B|| = \sqrt{(A_1-B_1)^2 +(A_2-B_2)^2... (A_n-B-n)^2 }
$$

where n is the number of components in the vectors. 

</aside>

$$
V_1 - V_2 = \begin{bmatrix}2 \\ 3 \\ 1 \end{bmatrix} - \begin{bmatrix}-1 \\ 3 \\ -2 \end{bmatrix} = \begin{bmatrix}3 \\ 0 \\ 3 \end{bmatrix}
$$

$$
||V_1-V_2|| = \sqrt{3^2+0^2+3^2} = \sqrt{18} = 3\sqrt{2}
$$

## Answer:

<aside>
‚úÖ The distance between the two vectors is $3\sqrt{2}$

</aside>

---

# 10. (2.6.1) ‚ùì

> ‚ùì Show that the following is Hermitian:
> 
> 
> $$
> \begin{bmatrix}5 & 4+5i & 6-16i \\ 4-5i & 13 & 7 \\ 
> 6+16i & 7 & -2.1 \end{bmatrix}
> $$
> 

<aside>
üí° Reminder:  a matrix is a Hermitian matrix, if the original is equal to the conjugate transpose: 

ex:

$$
M = M^\dagger = \overline{M}^T
$$

</aside>

## Step 1: Take conjugate:

$$
\begin{bmatrix}5 & 4+5i & 6-16i \\ 4-5i & 13 & 7 \\ 
6+16i & 7 & -2.1 \end{bmatrix}^* = \begin{bmatrix}5 & 4-5i & 6+16i \\ 4+5i & 13 & 7 \\ 
6-16i & 7 & -2.1 \end{bmatrix} 
$$

## Step 2: Take Transpose:

$$
\begin{bmatrix}5 & 4-5i & 6-16i \\ 4-5i & 13 & 7 \\ 
6-16i & 7 & -2.1 \end{bmatrix} ^T = 
\begin{bmatrix}5 & 4-5i & 6+16i \\ 4+5i & 13 & 7 \\ 
6-16i & 7 & -2.1 \end{bmatrix} 
$$

### So $M^\dagger:$

$$
\begin{bmatrix}5 & 4-5i & 6+16i \\ 4+5i & 13 & 7 \\ 
6-16i & 7 & -2.1 \end{bmatrix} 
$$

## Step 3: Compare

$$
\begin{bmatrix}5 & 4-5i & 6+16i \\ 4+5i & 13 & 7 \\ 
6-16i & 7 & -2.1 \end{bmatrix}  = \begin{bmatrix}5 & 4-5i & 6+16i \\ 4+5i & 13 & 7 \\ 
6-16i & 7 & -2.1 \end{bmatrix} 
$$

## Answer:

<aside>
‚úÖ The original is equal to its conjugate transpose (or its dagger) therefore the matrix is Hermitian

</aside>

---

# 11. (2.6.1) ‚ùì

> ‚ùì Is the following matrix a Hermitian matrix? Show your work.
> 
> 
> $$
> \begin{bmatrix}3i & 2+2i \\ 
> 2-2i & 1 \\ 
> \end{bmatrix}
> $$
> 

<aside>
‚ÑπÔ∏è Before doing any work it is obvious that the matrix is not a Hermitian Matrix. 

Remember a Matrix is Hermitian if its conjugate transpose is equal to the original matrix. 

The conjugate of a matrix reverses the sign of all imaginary components 

Therefore is there are any imaginary components along the main diagonal (i.e. $\{M_{1,1} \;,\; M_{2,2} \;... M_{n,n}\} \;$ ) the matrix cannot be Hermitian.

</aside>

we will show this is true: 

## Step 1: Take conjugate:

$$
\begin{bmatrix}3i & 2+2i \\ 
2-2i & 1 \\ 
\end{bmatrix}^* = \begin{bmatrix}-3i & 2-2i \\ 
2+2i & 1 \\ 
\end{bmatrix}
$$

## Step 2: Take Transpose:

$$
\begin{bmatrix}-3i & 2-2i \\ 
2+2i & 1 \\ 
\end{bmatrix}^T = \begin{bmatrix}-3i & 2+2i \\ 
2-2i & 1 \\ 
\end{bmatrix}
$$

## Step 3: Compare

$$
\begin{bmatrix}3i & 2+2i \\ 
2-2i & 1 \\ 
\end{bmatrix} \neq \begin{bmatrix}-3i & 2+2i \\ 
2-2i & 1 \\ 
\end{bmatrix}
$$

## Answer:

<aside>
‚úÖ As we have show this matrix is not Hermitian, due to its having an imaginary number across the main diagonal

</aside>

---

# 12. (2.6.3) ‚ùì

> ‚ùì Is the following matrix a Unitary matrix? Show your work.
> 
> 
> $$
> {1 \over \sqrt{3}}
> \begin{bmatrix} 1+i & -1\\ 
> 1 & 1-i
> \end{bmatrix}
> $$
> 

<aside>
‚ÑπÔ∏è Formula:

A Matrix is Unitary if its inverse is equal to its Transpose Conjugate.

I/E:

$$
M^\dagger = M^{-1}
$$

Another way of saying this is, the matrix is unitary if the product of the matrix and its conjugate transpose is equal to the identity matrix

I/E:

$$
M \; M^\dagger = I
$$

These two statements are equivelant since $M \; M^{-1} = I$

</aside>

## Step 1: Inverse of $M$:

<aside>
‚ÑπÔ∏è There are two ways of calculating inverse: 

1: augment with the identity than row reduce until you‚Äôve reached the identity matrix on the left side. The resulting matrix on the right side is  the inverse 

2: use:

$$
U^{-1} = {1\over(Det(U))} * Adj(U)
$$

For a 2x2 matrix this is: 

$$
A^{-1} = {1 \over ad-bc}\begin{bmatrix}d&-b\\-c&a \end{bmatrix}
$$

</aside>

For this problem I believe the second version will be easier. 

$$
{1 \over ad-bc} = {1 \over (1+i)(1-i) -(1)(-1)} =  {1 \over 2 + 1}= {1 \over 3}
$$

$$
\begin{bmatrix}d&-b\\-c&a \end{bmatrix} = \begin{bmatrix} 1-i & 1\\ 
-1 & 1+i
\end{bmatrix}
$$

$$
{{1 \over \sqrt{3}}}\bigg({1 \over 3}\bigg){ \begin{bmatrix} 1-i & 1\\ 
-1 & 1+i
\end{bmatrix}}
$$

## Step 2: Transpose of $M$:

$$
{1 \over \sqrt{3}}
\begin{bmatrix} 1+i & -1\\ 
1 & 1-i
\end{bmatrix}^T = 

{1 \over \sqrt{3}}
\begin{bmatrix} 1+i & 1\\ 
-1 & 1-i
\end{bmatrix}
$$

## Step 3: Conjugate of $M^T$:

$$
{1 \over \sqrt{3}}
\begin{bmatrix} 1+i & 1\\ 
-1 & 1-i
\end{bmatrix}^* = 

{1 \over \sqrt{3}}
\begin{bmatrix} 1-i & 1\\ 
-1 & 1+i
\end{bmatrix}
$$

### $M^\dagger:$

$$
{1 \over \sqrt{3}}
\begin{bmatrix} 1-i & 1\\ 
-1 & 1+i
\end{bmatrix}
$$

## Does $M^\dagger =M^{-1}$:

$$
M^{-1} = {{1 \over \sqrt{3}}}\bigg({1 \over 3}\bigg){ \begin{bmatrix} 1-i & 1\\ 
-1 & 1+i
\end{bmatrix}}
$$

$$
M^\dagger = {1 \over \sqrt{3}}
\begin{bmatrix} 1-i & 1\\ 
-1 & 1+i
\end{bmatrix}
$$

$$
{{1 \over \sqrt{3}}}\bigg({1 \over 3}\bigg){ \begin{bmatrix} 1-i & 1\\ 
-1 & 1+i
\end{bmatrix}} \neq  {1 \over \sqrt{3}}
\begin{bmatrix} 1-i & 1\\ 
-1 & 1+i
\end{bmatrix}
$$

<aside>
‚ùó It seems as if an easy way to determine if a matrix is NOT unitary is to find the Determinate of the matrix. 

If the Determinate is NOT 1, the matrix cannot be unitary.

</aside>

## Answer:

<aside>
‚úÖ No, the matrix is not unitary, as the complex conjugate does not equal the inverse of the matrix

</aside>

---

# 13. (2.7.5) ‚ùì

> ‚ùì Let $A = \begin{bmatrix}3 & 4 \end{bmatrix}$  and $B = \begin{bmatrix}
3 & 1 \\
2 & 4
 \end{bmatrix}$. Calculate $(A \otimes B)^\dagger$  and $A^\dagger \otimes B^\dagger$. Show that they are equal. ‚ùì
> 

<aside>
‚ÑπÔ∏è Tensor : $\otimes$ 

Tensor product is a way to calculate all of the different combinations between two vectors, matrixes, or a combination of the two.

with 1x2 matrix:

$$
\begin{bmatrix} a  \\ b\end{bmatrix} \otimes \begin{bmatrix} c  \\ d\end{bmatrix} = 
\begin{bmatrix}  a\begin{bmatrix} c  \\ d\end{bmatrix} \\ b\begin{bmatrix} c  \\ d\end{bmatrix}  \end{bmatrix}
$$

</aside>

## $(A \otimes B)^\dagger$ :

$$
 \begin{bmatrix}3 & 4 \end{bmatrix}  \otimes  \begin{bmatrix}
3 & 1 \\
2 & 4
 \end{bmatrix} = \begin{bmatrix}3 \begin{bmatrix}
3 & 1 \\
2 & 4
 \end{bmatrix}& 4 \begin{bmatrix}
3 & 1 \\
2 & 4
 \end{bmatrix}\end{bmatrix} =  \begin{bmatrix}
9 & 3 & 9 & 1 \\
6 & 12 & 8 & 16
 \end{bmatrix} 
$$

$$
\begin{bmatrix}
9 & 3 & 9 & 1 \\
6 & 12 & 8 & 16
 \end{bmatrix} ^\dagger: \begin{bmatrix}
9 & 6 \\
3 & 12 \\
9 & 8 \\ 
1 & 16
 \end{bmatrix}\rightarrow \begin{bmatrix}
9 & 6 \\
3 & 12 \\
9 & 8 \\ 
1 & 16
 \end{bmatrix}
$$

There was no change from the transpose to the conjugate step due to the non-existence of imaginary numbers in the matrix

## $A^\dagger \otimes B^\dagger :$

$$
A^\dagger = \begin{bmatrix} 3 \\ 4\end{bmatrix}
$$

$$
B^\dagger = \begin{bmatrix}  3 & 2 \\ 1 & 4\end{bmatrix}
$$

again for both matrixes, since the matrix consists entirely of real numbers the conjugate changes nothing, therefore finding the dagger is equivalent to finding the Transpose. 

$$
\begin{bmatrix} 3 \\ 4\end{bmatrix} \otimes  \begin{bmatrix}  3 & 2 \\ 1 & 4\end{bmatrix} = \begin{bmatrix} 3 \begin{bmatrix}  3 & 2 \\ 1 & 4\end{bmatrix} \\ 4\begin{bmatrix}  3 & 2 \\ 1 & 4\end{bmatrix} \end{bmatrix}  = \begin{bmatrix}
9 & 6 \\
3 & 12 \\
9 & 8 \\ 
1 & 16
 \end{bmatrix}
$$

## Compare:

$$
(A \otimes B)^\dagger= \begin{bmatrix}
9 & 6 \\
3 & 12 \\
9 & 8 \\ 
1 & 16
 \end{bmatrix}
$$

$$
A^\dagger \otimes B^\dagger =\begin{bmatrix}
9 & 6 \\
3 & 12 \\
9 & 8 \\ 
1 & 16
 \end{bmatrix}
$$

$$
\begin{bmatrix}
9 & 6 \\
3 & 12 \\
9 & 8 \\ 
1 & 16
 \end{bmatrix} = \begin{bmatrix}
9 & 6 \\
3 & 12 \\
9 & 8 \\ 
1 & 16
 \end{bmatrix}
$$

Therefore: 

$$
(A \otimes B)^\dagger= A^\dagger \otimes B^\dagger
$$

## Answer:

<aside>
‚úÖ We have shown that $(A \otimes B)^\dagger= A^\dagger \otimes B^\dagger$.

</aside>